\documentclass[12pt]{article}

\usepackage[a4paper,margin=2cm]{geometry}
\usepackage{amsmath, amssymb, amsthm, amsfonts, tikz, algpseudocode}
\usepackage[plain]{algorithm}
\usepackage[framemethod=default]{mdframed}

\theoremstyle{plain}
\newtheorem*{theorem}{Theorem}
\newtheorem*{lemma}{Lemma}
\newtheorem*{claim}{Claim}
\newtheorem*{definition}{Definition}
\newtheorem*{corollary}{Corollary}
\newtheorem*{remark}{Remark}
\newtheorem*{proposition}{Proposition}
\DeclareMathOperator*{\argmin}{arg\,min}
\DeclareMathOperator*{\eig}{eig}
\DeclareMathOperator*{\diag}{diag}
\DeclareMathOperator*{\vol}{Vol}

%%%% TITLE

\title{Math 690: Topics in Data Analysis and Computation \\
Lecture notes for October 5, 2017}
\date{}

\author{Scribed by Dev Dabke and Andrew Cho}

\begin{document}
\maketitle

\section{Consistency of Spectral Clustering}

\subsection{The Problem Setup}

Suppose $ X_{i} \sim P $ where $ P $ is some distribution on $ \Omega \subset \mathbb{R}^{D} $.

$ W_{ij} $ is the affinity matrix where, as an example,
\[
W_{ij} = e^{\frac{-|x_i - x_j|^2}{\varepsilon}}
\]
where $ \varepsilon > 0 $.
\\ \\
As $ n \to \infty $, we want to show the convergence of the graph Laplacian $ \mathcal{L} $.
\begin{enumerate}
  \item $ \mathcal{L}_{n} = D - W $ where $ D_{ij} = \sum_{j = 1}^{n} W_{ij} $ ($  \to U $), i.e.\ unnormalized
  \item $ \mathcal{L}_{n}' = D^{-\frac{1}{2}} (D - W) D^{-\frac{1}{2}} $ where ($  \to U' $), i.e.\ symmetric
  \item $ \mathcal{L}_{n}'' = D^{-1} (D - W) = I - P $, i.e.\ random walk
\end{enumerate}

\subsection{$ U $}

Here, note that
\begin{align*}
  U &: C(\Omega) \to C(\Omega) \\
  Uf(x) &= f(x)d(x) - \int k(x, y) f(y) dP(y)
\end{align*}
where
\begin{align*}
  dP(x) &= p(x)dx \\
  d(x) &= \int k(x, y) dP(y) \\
  x \in \Omega
\end{align*}

\subsection{$ U' $}

Here
\[
U' f(x) = f(x) - \int{ \frac{ k(x, y) }{ \sqrt{ d(x) } \sqrt{ d(y) } } f(y) dP(y) }
\]

\begin{proof}

  \begin{align*}
    (D^{-\frac{1}{2}} W D^{-\frac{1}{2}})_{ij} &= \frac{1}{\sqrt{D_{ii}}} W_{ij} \frac{1}{\sqrt{D_{jj}}} \\
    &= \frac{ \frac{1}{n} k(x_i, x_j) }{ \sqrt{ \frac{1}{n} \sum_{j'} k(x_i, x_j') } \sqrt{ \frac{1}{n} \sum_{j'} k(x_j, x_j') } } \\
    &\approx \frac{ \frac{1}{n} k(x_i, x_j) }{ \sqrt{d(x_i)} \sqrt{d(x_j)} } \\
  \end{align*}

\end{proof}

\subsection{First $ r $ spectral convergence}

\end{document}
